* Q1
** 
* Q2
** If a, b \in Z(R) then a - b \in Z(R) and ab \in Z(R) 
** Notice ab = ba 
*** Now let c \in R
*** (ab)c = (ba)c = b(ac) = a(bc) = a(cb) = (ac)b = c(ab) So ab \in Z(R)
*** (a-b)c = ac - bc = ca - cb = c(a-b) so a-b \in Z(R)
** So Z(R) is a subring of R
* Q3
** Notice that the only idempotent elements in Z are 0 and 1
** So the set of idempotent elements in Z^n is {(a_1, a_2, ... ,a_n) | a_i \in {0, 1}} 
* Q4
** Consider r \in R and x + y \in I + J
*** So r(x + y) = rx + ry
*** Clearly rx \in I and rj \in J so rx + ry \in I + J
*** So I + J is an ideal
* Q5
** Let x \in IJ be x = a_{1}b_{1} + ... + a_{n}b_{n}
*** So r \in R rx = ra_{1}b_{1} + ... + ra_{n}b_{n}
*** Since any ra_{i}b_{i} is in I or J then rx \in IJ 
* Q6
** 
* Q7
** <a> = {ras | r,s \in R}
** R is commutative then <a> = {ra | r \in R} principal ideal
* Q11
** Consider Z[X]/P 
** 0 in this ring is any polynomial with all even coefficient
** Let a, b \in Z[X]/P be non-zero
** So both a and b have some odd coefficient
* Homomorphism
** Q12
*** Let s \in S, s = \phi(r) with r \in R
*** \phi(r)\phi(a) = s\phi(a) = \phi(ra)
** Q17
*** Result from course F[X]/<f> \cong F(a) if a \in E and extension of F and f is min. polynomial a over F
** Q24
*** Let \phi: S \to (S + I)/I be \phi(s) = s + I
**** Notice that this is a composition of two homomorphisms
***** S \to S + I
***** S + I \to (S + I)/I
*** As a composition of homomorphisms \phi is a homomorphism
*** Note that \phi is surjective
*** In fact if x + I \in (S + I)/I then by definition x = s + a with s \in S and a \in I
*** So \phi(s) = s + I = s + a + I = x + I
*** Notice x \in Ker(\phi) iff x \in I
*** So Ker(\phi) = S \cap I
*** So by the first isomorphism theorem \phi_bar: S/(S \cap I) \to (S + I)/I is an isomorphism defined by \phi_bar(s + S \cap I) = \phi(s) = s + I
* Polynomial Rings
** Q25
*** If x - a is a factor of f(x) then f(x) = (x - a)g(x)
**** So f(a) = (a - a)g(x) = 0g(x) = 0
**** So a is a zero of f(x)
*** If a is a zero of f(x)
**** Then by the remainder theorem f(a) = 0 is a remainder of f(x)/(x - a)
**** So (x - a) | f(x)
**** So (x - a) is a factor of f(x)
** 26
*** 
** Q27
*** Let \phi: R \to R/I be the natural quotient map
**** Then we have \phi_bar: R[X] \to (R/I)[X]
**** Certainly \phi_bar is surjective
**** If f \in R[X] then f \in Ker(\phi_bar) iff f \sum_{i \in N_0} IX^i
**** So for all a_i + I, a_i \in I
**** As kernels are Ideals we have I[X] is an ideal
**** By The First Isomorphism Theorem 
** Q36
*** Clearly X^{2p} - 1 = (X^P - 1)(X^p + 1) as X^2p - 1 is the difference of two squares
*** We know X^p - 1 = (X - 1)\phi_p(X) = \phi_{1}\phi_p
*** By replaceing X with -X we have
**** -(X^p + 1) = (-X)^p - 1 = (-X - 1)\phi_p(-X) = -(X + 1)\phi_p(-X)
* EDs, PIDs, and UFDs
** Q41
*** We know F[X] must be an integral domain
*** Let I be an ideal of F[X]
*** If I = {0} then I = <0>
*** If I \ne <0> then let g(x) \in I have minimal degree
*** So <g(x)> \sub I
*** Now let f(x) \in I
*** We have f(x) = q(x)g(x) + r(x) with r(x) = 0 or deg(r(x)) \lt deg(g(x))
*** So r(x) = f(X) - q(x)g(x) \in I
*** This contradicts the minimality of g(x)
*** So r(x) must be zero
*** So <g(x)> = I
*** F[X] is a UFD because all PIDs are UFDs
** Q42
*** Assume <f> is not maximal
**** So there must be some non-zero non-unit g such that <f> \sub <g> \sub R
**** so f = rg for some r \in R
**** Since f is irreducible r must be a unit
**** So r^{-1}f = g but this implies <g> \sub <f> a contradiction
**** So r cannot be a unit but this contradicts the irreducibility of f
*** A similiar argument follows for the other direction
** Q43
*** Let \phi: R \to S be a surjective ring homomorphism and R a PID
*** Let J \sub S be an Ideal of S
*** So \phi^-1(J) must be an Ideal of R call it <a>
*** So J = \phi(\phi^-1(J)) = \phi(<a>) = <\phi(a)>
*** So S is a PID
** Q45
*** 
** Q51
*** Let d(g) \le d(h) for all h \in I
*** Since this is a Euclidean Domain, h = qg + r with r = 0 or d(r) \lt d(g)
*** If r \ne 0 then r = h - qg \in I
*** But this contradicts the minimality of g
*** So g | h and I = <g>
* Fields
** Q52
*** Remember that for finite fields of order q a^q = a for all a \in F
*** So for all a \in F f(a) = a^q - a = a - a = 0
*** So all elements of F are factors of X^q - X
*** So X^q - X = (X - a_1)...(X- a_q)
*** So this is a splitting field
** Q53
*** Notice F_3 has charateritic 3 so a^3 = a for all  a \in F_3
*** So a^3 - a = 0 for all a \in F_3
*** So we have an artin-schrier polynomial X^3 - X + 1 \in F_3[X]
*** So F_9 = F_3[X]/<X^3 - X + 1>
*** Let \alpha = X + <X^3 - X + 1>
*** Notice \alpha^3 = (X + <X^3 - X + 1>)^3 = X^3 + <X^3 - X + 1> = X + <X^3 -X + 1> = \alpha
*** So F_9 = {a\alpha^2 + b\alpha + c | a,b,c \in F_3}
*** Consider (a\alpha^2 + b\alpha + c)^3 = a\alpha^6 + b\alpha^4 + c^3 = a\alpha^2 + b\alpha^2 + c = (a + b)\alpha^2 + c 
*** So we have teh cube of each element in F_27 has no alpha term of degree 1
*** So X^3 - \alpha has no zeroes in F_27
*** So F_27/<X^3 - \alpha> is a field of size 9^3
** Q54
*** Notice That x \in F is x = a + bi/c + di with a,b,c,d \in Z
*** a + bi/c + di = (a + bi)(c - di)/c^2 + d^2 = ac + bd/c^2 + bc - ad/c^2 + d^2 i \in Q(i)
*** Now if y \in Q(i) is m/n + p/qi = mq + pni/nq \in F
*** So these are the same sets. So these fields are isomorphic
** Q55
*** Let X = (1 + 5^{1/2})^{1/2}
*** So X^2 = 1 + 5^{1/2}
*** So X^2 - 1 = 5^{1/2}
*** So (X^2 - 1)^2 = 5
*** So X^2 - 2X + 1 = 5
*** So X^2 - 2X - 4 = 0
*** Use mod p irreducibility test with p = 3
*** The degree is 4 as is the degree of the minimal polynomial
** Q56
*** First claim Q(2^{1/3} + 4^{1/3}) = Q(2^{1/3}, 4^{1/3})
*** Q(2^{1/3} + 4^{1/3}) \sub Q(2^{1/3}, 4^{1/3}) is clear
*** Then find [Q(2^{1/3}, 4^{1/3}):Q] = [Q(2^{1/3}):Q(4^{1/3})][Q(4^{1/3}):Q]
*** Find some polynomial of that degree that its a zero of
** Q58
*** 
** Q59
*** So the basis for F is {1_F, a} with a \in F
*** So x^2 = (-b)x + (-c)1
*** So x^2 + bx + c = 0
*** Quadratic formula for x
*** F must be equal to Q(x)
** Q60
*** If \alpha \in E is a zero of f then (x - \alpha) is a factor of F
*** 
** Q61
*** i
**** Notice X^4 - 6X^2 - 7 = (X^2 - 7)(X^2 + 1)
**** So 7^{1/2} and i are zeros of this polynomial
**** So 
*** ii
**** So [Q(7^{1/2}, i):Q] = [Q(7^{1/2}):Q(i)][Q(i):Q]
**** X^2 - 7 \in Q[i] has 7^{1/2} as a zero and (X - 1)(X + 7) \ne X^2 - 7 and (X + 1)(X - 7) \ne x^2 - 7
**** So this polynomial is irreducible so it is the min polynomial over Q(i)
**** [Q(7^{1/2}):Q(i)] = 2
**** Consider X^2 + 1 \in Q[X]
**** i^2 + 1 = -1 + 1 = 0 and X^2 + 1 does not factor in Q[X]
**** So [Q(i):Q] = 2
**** [Q(7^{1/2}, i):Q] = [Q(7^{1/2}):Q(i)][Q(i):Q] = 2 * 2 = 4
** Q62
*** Notice a = (a^{1/2})(a^{1/2}) so a \in Q(a^{1/2}) so Q(a) \sub Q (a^{1/2})
*** Notice a^{1/2} = 1 + a so a^{1/2} \in Q(a) so Q(a^{1/2}) \sub Q(a)
